proof performance experiments with @nikswamy

src/tls/Parsers.Ticket.Low.fst
@@ -48,15 +48,59 @@ let write_boolean =
     (fun x -> synth_boolean_inv x)
     ()
 
-let valid_ticketContents12_intro h input pos =
+val valid_ticketContents12_intro'
+  (h: HS.mem)
+  (input: LP.slice)
+  (pos: U32.t)
+: Lemma
+  (requires (
+    LP.valid protocolVersion_parser h input pos /\ (
+    let pos1 = LP.get_valid_pos protocolVersion_parser h input pos in
+    LP.valid cipherSuite_parser h input pos1 /\ (
+    let pos2 = LP.get_valid_pos cipherSuite_parser h input pos1 in
+    LP.valid boolean_parser h input pos2 /\ (
+    let pos3 = LP.get_valid_pos boolean_parser h input pos2 in
+    LP.valid (LPB.parse_flbytes 48) h input pos3 /\ (
+    let pos4 = LP.get_valid_pos (LPB.parse_flbytes 48) h input pos3 in
+    LP.valid LPI.parse_u32 h input pos4 /\ (
+    let pos5 = LP.get_valid_pos LPI.parse_u32 h input pos4 in
+    LP.valid LPI.parse_u32 h input pos5
+  )))))))
+  (ensures (
+    let pos1 = LP.get_valid_pos protocolVersion_parser h input pos in
+    let pos2 = LP.get_valid_pos cipherSuite_parser h input pos1 in
+    let pos3 = LP.get_valid_pos boolean_parser h input pos2 in
+    let pos4 = LP.get_valid_pos (LPB.parse_flbytes 48) h input pos3 in
+    let pos5 = LP.get_valid_pos LPI.parse_u32 h input pos4 in
+    let pos6 = LP.get_valid_pos LPI.parse_u32 h input pos5 in
+    LP.valid_content_pos ticketContents12_parser h input pos
+      ({
+        pv = LP.contents protocolVersion_parser h input pos;
+        Parsers.TicketContents12.cs = LP.contents cipherSuite_parser h input pos1;
+        ems = LP.contents boolean_parser h input pos2;
+        master_secret = LP.contents (LPB.parse_flbytes 48) h input pos3;
+        foo1 = LP.contents LPI.parse_u32 h input pos4;
+        foo2 = LP.contents LPI.parse_u32 h input pos5;
+      })
+      pos6
+  ))
+
+let allow_inversion_tuple2 (t1 t2: Type) : Lemma (inversion (tuple2 t1 t2)) [SMTPat (tuple2 t1 t2)] = allow_inversion (tuple2 t1 t2)
+
+#reset-options "--z3rlimit 128 --z3refresh --log_queries --query_stats --max_fuel 0 --initial_ifuel 0 --max_ifuel 0 --using_facts_from '* -LowParse.Spec.Combinators.nondep_then'"
+
+let valid_ticketContents12_intro' h input pos =
+  synth_ticketContents12_injective ();
   LP.valid_synth h ticketContents12'_parser synth_ticketContents12 input pos;
+  LP.valid_nondep_then h (protocolVersion_parser `LP.nondep_then` cipherSuite_parser `LP.nondep_then` boolean_parser `LP.nondep_then` ticketContents12_master_secret_parser `LP.nondep_then` LPI.parse_u32) LPI.parse_u32 input pos;
+  LP.valid_nondep_then h (protocolVersion_parser `LP.nondep_then` cipherSuite_parser `LP.nondep_then` boolean_parser `LP.nondep_then` ticketContents12_master_secret_parser) LPI.parse_u32 input pos;
   LP.valid_nondep_then h (protocolVersion_parser `LP.nondep_then` cipherSuite_parser `LP.nondep_then` boolean_parser) ticketContents12_master_secret_parser input pos;
   LP.valid_nondep_then h (protocolVersion_parser `LP.nondep_then` cipherSuite_parser) boolean_parser input pos;
   LP.valid_nondep_then h protocolVersion_parser cipherSuite_parser input pos
 
-#reset-options "--z3rlimit 256 --max_ifuel 8 --initial_ifuel 8 --max_fuel 2 --z3cliopt smt.arith.nl=false --using_facts_from '* -FStar.Tactics -FStar.Reflection'"
+// #reset-options "--z3rlimit 256 --max_ifuel 8 --initial_ifuel 8 --max_fuel 2 --z3cliopt smt.arith.nl=false --using_facts_from '* -FStar.Tactics -FStar.Reflection'"
 
-let valid_ticketContents13_intro h input pos =
+let valid_ticketContents13_intro' h input pos =
   let cs = LP.contents cipherSuite_parser h input pos in
   let pos1 = LP.get_valid_pos cipherSuite_parser h input pos in
   let rms = LP.contents ticketContents13_rms_parser h input pos1 in
