src/tls/Parsers11.fst
@@ -1,0 +1,61 @@
+module Parsers11
+open Parsers.ProtocolVersion
+open Parsers.CipherSuite
+open Parsers.Boolean
+open Parsers.TicketContents11
+
+module HS = FStar.HyperStack
+module LP = LowParse.Low
+module LPT = LowParse.SLow.Tac.Enum
+module LPB = LowParse.Spec.Bytes
+module U32 = FStar.UInt32
+module LPI = LowParse.Spec.Int
+
+friend Parsers.ProtocolVersion
+friend Parsers.CipherSuite
+friend Parsers.Boolean
+friend Parsers.TicketContents11
+
+val valid_ticketContents12_intro'
+  (h: HS.mem)
+  (input: LP.slice)
+  (pos: U32.t)
+: Lemma
+  (requires (
+    LP.valid protocolVersion_parser h input pos /\ (
+    let pos1 = LP.get_valid_pos protocolVersion_parser h input pos in
+    LP.valid cipherSuite_parser h input pos1 /\ (
+    let pos2 = LP.get_valid_pos cipherSuite_parser h input pos1 in
+    LP.valid boolean_parser h input pos2 /\ (
+    let pos3 = LP.get_valid_pos boolean_parser h input pos2 in
+    LP.valid (LPB.parse_flbytes 48) h input pos3 /\ (
+    let pos4 = LP.get_valid_pos (LPB.parse_flbytes 48) h input pos3 in
+    LP.valid LPI.parse_u32 h input pos4
+  ))))))
+  (ensures (
+    let pos1 = LP.get_valid_pos protocolVersion_parser h input pos in
+    let pos2 = LP.get_valid_pos cipherSuite_parser h input pos1 in
+    let pos3 = LP.get_valid_pos boolean_parser h input pos2 in
+    let pos4 = LP.get_valid_pos (LPB.parse_flbytes 48) h input pos3 in
+    let pos5 = LP.get_valid_pos LPI.parse_u32 h input pos4 in
+    LP.valid_content_pos ticketContents11_parser h input pos
+      ({
+        pv = LP.contents protocolVersion_parser h input pos;
+        Parsers.TicketContents11.cs = LP.contents cipherSuite_parser h input pos1;
+        ems = LP.contents boolean_parser h input pos2;
+        master_secret = LP.contents (LPB.parse_flbytes 48) h input pos3;
+        foo1 = LP.contents LPI.parse_u32 h input pos4;
+      })
+      pos5
+  ))
+
+let allow_inversion_tuple2 (t1 t2: Type) : Lemma (inversion (tuple2 t1 t2)) [SMTPat (tuple2 t1 t2)] = allow_inversion (tuple2 t1 t2)
+
+#reset-options "--z3rlimit 10 --z3refresh --log_queries --query_stats --max_fuel 0 --initial_ifuel 0 --max_ifuel 0 --using_facts_from '* -LowParse.Spec.Combinators.nondep_then -LowParse.Spec.Combinators.parse_synth -LowParse.Spec.Combinators.and_then'"
+
+let valid_ticketContents12_intro' h input pos =
+  LP.valid_synth h ticketContents11'_parser synth_ticketContents11 input pos;
+  LP.valid_nondep_then h (protocolVersion_parser `LP.nondep_then` cipherSuite_parser `LP.nondep_then` boolean_parser `LP.nondep_then` ticketContents11_master_secret_parser) LPI.parse_u32 input pos;
+  LP.valid_nondep_then h (protocolVersion_parser `LP.nondep_then` cipherSuite_parser `LP.nondep_then` boolean_parser) ticketContents11_master_secret_parser input pos;
+  LP.valid_nondep_then h (protocolVersion_parser `LP.nondep_then` cipherSuite_parser) boolean_parser input pos;
+  LP.valid_nondep_then h protocolVersion_parser cipherSuite_parser input pos
