src/tls/Parsers9.fst
@@ -1,0 +1,54 @@
+module Parsers9
+open Parsers.ProtocolVersion
+open Parsers.CipherSuite
+open Parsers.TicketContents9
+
+module HS = FStar.HyperStack
+module LP = LowParse.Low
+module LPT = LowParse.SLow.Tac.Enum
+module LPB = LowParse.Spec.Bytes
+module U32 = FStar.UInt32
+module LPI = LowParse.Spec.Int
+
+friend Parsers.ProtocolVersion
+friend Parsers.CipherSuite
+friend Parsers.TicketContents9
+
+val valid_ticketContents12_intro'
+  (h: HS.mem)
+  (input: LP.slice)
+  (pos: U32.t)
+: Lemma
+  (requires (
+    LP.valid protocolVersion_parser h input pos /\ (
+    let pos1 = LP.get_valid_pos protocolVersion_parser h input pos in
+    LP.valid cipherSuite_parser h input pos1 /\ (
+    let pos2 = LP.get_valid_pos cipherSuite_parser h input pos1 in
+    LP.valid LPI.parse_u32 h input pos2 /\ (
+    let pos3 = LP.get_valid_pos LPI.parse_u32 h input pos2 in
+    LP.valid (LPB.parse_flbytes 48) h input pos3
+  )))))
+  (ensures (
+    let pos1 = LP.get_valid_pos protocolVersion_parser h input pos in
+    let pos2 = LP.get_valid_pos cipherSuite_parser h input pos1 in
+    let pos3 = LP.get_valid_pos LPI.parse_u32 h input pos2 in
+    let pos4 = LP.get_valid_pos (LPB.parse_flbytes 48) h input pos3 in
+    LP.valid_content_pos ticketContents9_parser h input pos
+      ({
+        pv = LP.contents protocolVersion_parser h input pos;
+        Parsers.TicketContents9.cs = LP.contents cipherSuite_parser h input pos1;
+        ems = LP.contents LPI.parse_u32 h input pos2;
+        master_secret = LP.contents (LPB.parse_flbytes 48) h input pos3;
+      })
+      pos4
+  ))
+
+let allow_inversion_tuple2 (t1 t2: Type) : Lemma (inversion (tuple2 t1 t2)) [SMTPat (tuple2 t1 t2)] = allow_inversion (tuple2 t1 t2)
+
+#reset-options "--z3rlimit 128 --z3refresh --log_queries --query_stats --max_fuel 0 --initial_ifuel 0 --max_ifuel 0"
+
+let valid_ticketContents12_intro' h input pos =
+  LP.valid_synth h ticketContents9'_parser synth_ticketContents9 input pos;
+  LP.valid_nondep_then h (protocolVersion_parser `LP.nondep_then` cipherSuite_parser `LP.nondep_then` LPI.parse_u32) ticketContents9_master_secret_parser input pos;
+  LP.valid_nondep_then h (protocolVersion_parser `LP.nondep_then` cipherSuite_parser) LPI.parse_u32 input pos;
+  LP.valid_nondep_then h protocolVersion_parser cipherSuite_parser input pos
